% Equation 1
\begin{dmath}
{{c}}_{t}={c1}\, {{c}}_{t+1}+\left(1-{c1}\right)\, {{c}}_{t-1}-{c2}\, \left({{r}}_{t}-{{\pi}}_{t+1}-{{\varepsilon_b}}_{t}\right)
\end{dmath}
% Equation 2
\begin{dmath}
{{i}}_{t}={i1}\, {{i}}_{t-1}+\left(1-{i1}\right)\, {{i}}_{t+1}+{i2}\, {{q}}_{t}+{{\varepsilon_q}}_{t}
\end{dmath}
% Equation 3
\begin{dmath}
{{q}}_{t}={q1}\, {{r^{k}}}_{t+1}-\left({{r}}_{t}-{{\pi}}_{t+1}-{{\varepsilon_b}}_{t}\right)+\left(1-{q1}\right)\, {{q}}_{t+1}
\end{dmath}
% Equation 4
\begin{dmath}
{{y}}_{t}={{c}}_{t}\, {ccy}+{{i}}_{t}\, {ciy}+{cvy}\, {{v}}_{t}+{{\varepsilon_g}}_{t}
\end{dmath}
% Equation 5
\begin{dmath}
{{y}}_{t}={cpsip}\, \left({calpha}\, {{k}}_{t}+\left(1-{calpha}\right)\, {{n}}_{t}+{{\varepsilon_a}}_{t}\right)
\end{dmath}
% Equation 6
\begin{dmath}
{{\pi}}_{t}-{cgammap}\, {{\pi}}_{t-1}={pi1}\, \left({{\pi}}_{t+1}-{{\pi}}_{t}\, {cgammap}\right)-{pi2}\, \left(100\, {{\varepsilon_p}}_{t}-{{mc}}_{t}\right)
\end{dmath}
% Equation 7
\begin{dmath}
{{mc}}_{t}=\left(1-{calpha}\right)\, {{w}}_{t}+{calpha}\, {{r^{k}}}_{t}-{{\varepsilon_a}}_{t}
\end{dmath}
% Equation 8
\begin{dmath}
{{\pi}}_{t}+{{w}}_{t}-{{w}}_{t-1}={{\pi}}_{t-1}\, {cgammaw}+{cbeta}\, \left({{\pi}}_{t+1}+{{w}}_{t+1}-{{w}}_{t}-{{\pi}}_{t}\, {cgammaw}\right)-{w1}\, \left({comega}\, {{u}}_{t}-100\, {{\varepsilon_w}}_{t}\right)
\end{dmath}
% Equation 9
\begin{dmath}
{comega}\, {{u}}_{t}={{w}}_{t}-\left({{z}}_{t}+{{\varepsilon_s}}_{t}+{comega}\, {{e}}_{t}\right)
\end{dmath}
% Equation 10
\begin{dmath}
{comega}\, {{u^{n}}}_{t}=100\, {{\varepsilon_w}}_{t}
\end{dmath}
% Equation 11
\begin{dmath}
{{l}}_{t}={{u}}_{t}+{{e}}_{t}
\end{dmath}
% Equation 12
\begin{dmath}
{{z}}_{t}=\left(1-{cv}\right)\, {{z}}_{t-1}+\frac{{cv}}{1-\frac{{ch}}{{ctau}}}\, \left({{c}}_{t}-{{c}}_{t-1}\, \frac{{ch}}{{ctau}}\right)
\end{dmath}
% Equation 13
\begin{dmath}
{{\bar{k}}}_{t}={k1}\, {{\bar{k}}}_{t-1}+{{i}}_{t}\, \left(1-{k1}\right)+{{\varepsilon_q}}_{t}\, {k2}
\end{dmath}
% Equation 14
\begin{dmath}
{{k}}_{t}={{v}}_{t}+{{\bar{k}}}_{t-1}
\end{dmath}
% Equation 15
\begin{dmath}
{{v}}_{t}={{r^{k}}}_{t}\, \frac{1-{cpsi}}{{cpsi}}
\end{dmath}
% Equation 16
\begin{dmath}
{{k}}_{t}={{n}}_{t}+{{w}}_{t}-{{r^{k}}}_{t}
\end{dmath}
% Equation 17
\begin{dmath}
{{r}}_{t}={crhointr}\, {{r}}_{t-1}+\left(1-{crhointr}\right)\, \left({{\pi}}_{t}\, {crpi}+{cry}\, {{y^{gap}}}_{t}+{crdy}\, \left({{y^{gap}}}_{t}-{{y^{gap}}}_{t-1}\right)\right)-{{\varepsilon_r}}_{t}
\end{dmath}
% Equation 18
\begin{dmath}
{{e}}_{t}-{{e}}_{t-1}={cbeta}\, \left({{e}}_{t+1}-{{e}}_{t}\right)+{e1}\, \left({{n}}_{t}-{{e}}_{t}\right)
\end{dmath}
% Equation 19
\begin{dmath}
{cf}_{t}={c1}\, {cf}_{t+1}+\left(1-{c1}\right)\, {cf}_{t-1}-{c2}\, \left({rf}_{t}-{{\varepsilon_b}}_{t}\right)
\end{dmath}
% Equation 20
\begin{dmath}
{invf}_{t}={{\varepsilon_q}}_{t}+{i1}\, {invf}_{t-1}+\left(1-{i1}\right)\, {invf}_{t+1}+{i2}\, {qf}_{t}
\end{dmath}
% Equation 21
\begin{dmath}
{qf}_{t}={q1}\, {rkf}_{t+1}-\left({rf}_{t}-{{\varepsilon_b}}_{t}\right)+\left(1-{q1}\right)\, {qf}_{t+1}
\end{dmath}
% Equation 22
\begin{dmath}
{yf}_{t}={{\varepsilon_g}}_{t}+{ccy}\, {cf}_{t}+{ciy}\, {invf}_{t}+{cvy}\, {vf}_{t}
\end{dmath}
% Equation 23
\begin{dmath}
{yf}_{t}={cpsip}\, \left({{\varepsilon_a}}_{t}+{calpha}\, {kf}_{t}+\left(1-{calpha}\right)\, {nf}_{t}\right)
\end{dmath}
% Equation 24
\begin{dmath}
0=\left(1-{calpha}\right)\, {wf}_{t}+{calpha}\, {rkf}_{t}-{{\varepsilon_a}}_{t}
\end{dmath}
% Equation 25
\begin{dmath}
{wf}_{t}={{\varepsilon_s}}_{t}+{zf}_{t}+{comega}\, {nf}_{t}
\end{dmath}
% Equation 26
\begin{dmath}
{zf}_{t}=\left(1-{cv}\right)\, {zf}_{t-1}+\frac{{cv}}{1-\frac{{ch}}{{ctau}}}\, \left({cf}_{t}-\frac{{ch}}{{ctau}}\, {cf}_{t-1}\right)
\end{dmath}
% Equation 27
\begin{dmath}
{kbarf}_{t}={{\varepsilon_q}}_{t}\, {k2}+{k1}\, {kbarf}_{t-1}+\left(1-{k1}\right)\, {invf}_{t}
\end{dmath}
% Equation 28
\begin{dmath}
{kf}_{t}={vf}_{t}+{kbarf}_{t-1}
\end{dmath}
% Equation 29
\begin{dmath}
{vf}_{t}=\frac{1-{cpsi}}{{cpsi}}\, {rkf}_{t}
\end{dmath}
% Equation 30
\begin{dmath}
{kf}_{t}={nf}_{t}+{wf}_{t}-{rkf}_{t}
\end{dmath}
% Equation 31
\begin{dmath}
{ef}_{t}-{ef}_{t-1}={cbeta}\, \left({ef}_{t+1}-{ef}_{t}\right)+{e1}\, \left({nf}_{t}-{ef}_{t}\right)
\end{dmath}
% Equation 32
\begin{dmath}
{{y^{gap}}}_{t}={{y}}_{t}-{yf}_{t}
\end{dmath}
% Equation 33
\begin{dmath}
{{\varepsilon_b}}_{t}={crhob}\, {{\varepsilon_b}}_{t-1}+{{\eta_b}}_{t}
\end{dmath}
% Equation 34
\begin{dmath}
{{\varepsilon_q}}_{t}={crhoq}\, {{\varepsilon_q}}_{t-1}+{{\eta_q}}_{t}
\end{dmath}
% Equation 35
\begin{dmath}
{{\varepsilon_g}}_{t}={crhog}\, {{\varepsilon_g}}_{t-1}+{{\eta_g}}_{t}+{crhoga}\, {{\eta_a}}_{t}
\end{dmath}
% Equation 36
\begin{dmath}
{{\varepsilon_a}}_{t}={{\eta_a}}_{t}+{crhoa}\, {{\varepsilon_a}}_{t-1}
\end{dmath}
% Equation 37
\begin{dmath}
{{\varepsilon_p}}_{t}={crhop}\, {{\varepsilon_p}}_{t-1}+{{\eta_p}}_{t}-{cmup}\, {AUX\_EXO\_LAG\_54\_0}_{t-1}
\end{dmath}
% Equation 38
\begin{dmath}
{{\varepsilon_r}}_{t}={crhor}\, {{\varepsilon_r}}_{t-1}+{{\eta_r}}_{t}
\end{dmath}
% Equation 39
\begin{dmath}
{{\varepsilon_s}}_{t}={crhos}\, {{\varepsilon_s}}_{t-1}+{{\eta_s}}_{t}
\end{dmath}
% Equation 40
\begin{dmath}
{{\varepsilon_w}}_{t}={crhow}\, {{\varepsilon_w}}_{t-1}+{{\eta_w}}_{t}-{cmuw}\, {AUX\_EXO\_LAG\_56\_0}_{t-1}
\end{dmath}
% Equation 41
\begin{dmath}
{dyobs}_{t}={{y}}_{t}+{ctaubar}+{cebar}-{{y}}_{t-1}
\end{dmath}
% Equation 42
\begin{dmath}
{dcobs}_{t}={{c}}_{t}+{ctaubar}+{cebar}-{{c}}_{t-1}
\end{dmath}
% Equation 43
\begin{dmath}
{diobs}_{t}={{i}}_{t}+{ctaubar}+{cebar}-{{i}}_{t-1}
\end{dmath}
% Equation 44
\begin{dmath}
{piobs}_{t}={{\pi}}_{t}+{cpibar}
\end{dmath}
% Equation 45
\begin{dmath}
{dwobs}_{t}-{piobs}_{t}={{w}}_{t}+{ctaubar}-{{w}}_{t-1}-\left({{\pi}}_{t}-{{\pi}}_{t-1}\right)
\end{dmath}
% Equation 46
\begin{dmath}
{deobs}_{t}={{e}}_{t}+{cebar}-{{e}}_{t-1}
\end{dmath}
% Equation 47
\begin{dmath}
{uobs}_{t}={{u}}_{t}+{cubar}
\end{dmath}
% Equation 48
\begin{dmath}
{robs}_{t}=4\, {crbar}+{{r}}_{t}\, 4
\end{dmath}
% Equation 49
\begin{dmath}
{ryear}_{t}={{r}}_{t}\, 4
\end{dmath}
% Equation 50
\begin{dmath}
{piyear}_{t}={{\pi}}_{t}+{{\pi}}_{t-1}+{AUX\_ENDO\_LAG\_2\_1}_{t-1}+{AUX\_ENDO\_LAG\_2\_2}_{t-1}
\end{dmath}
% Equation 51
\begin{dmath}
{AUX\_ENDO\_LAG\_2\_1}_{t}={{\pi}}_{t-1}
\end{dmath}
% Equation 52
\begin{dmath}
{AUX\_ENDO\_LAG\_2\_2}_{t}={AUX\_ENDO\_LAG\_2\_1}_{t-1}
\end{dmath}
% Equation 53
\begin{dmath}
{AUX\_EXO\_LAG\_54\_0}_{t}={{\eta_p}}_{t}
\end{dmath}
% Equation 54
\begin{dmath}
{AUX\_EXO\_LAG\_56\_0}_{t}={{\eta_w}}_{t}
\end{dmath}
