% Equation 1
\begin{dmath}
{{c}}={{c}}\, {c1}+{{c}}\, \left(1-{c1}\right)-{c2}\, \left({{r}}-{{\pi}}-{epsilonb}\right)
\end{dmath}
% Equation 2
\begin{dmath}
{{i}}={{i}}\, {i1}+{{i}}\, \left(1-{i1}\right)+{i2}\, {{q}}+{epsilonq}
\end{dmath}
% Equation 3
\begin{dmath}
{{q}}={q1}\, {{r^{k}}}-\left({{r}}-{{\pi}}-{epsilonb}\right)+{{q}}\, \left(1-{q1}\right)
\end{dmath}
% Equation 4
\begin{dmath}
{{y}}={{c}}\, {ccy}+{{i}}\, {ciy}+{cvy}\, {{v}}+{epsilong}
\end{dmath}
% Equation 5
\begin{dmath}
{{y}}={cpsip}\, \left({calpha}\, {{k}}+\left(1-{calpha}\right)\, {{n}}+{epsilona}\right)
\end{dmath}
% Equation 6
\begin{dmath}
{{\pi}}-{{\pi}}\, {cgammap}=\left({{\pi}}-{{\pi}}\, {cgammap}\right)\, {pi1}-{pi2}\, \left(100\, {epsilonp}-{{mc}}\right)
\end{dmath}
% Equation 7
\begin{dmath}
{{mc}}=\left(1-{calpha}\right)\, {{w}}+{{r^{k}}}\, {calpha}-{epsilona}
\end{dmath}
% Equation 8
\begin{dmath}
{{\pi}}={{\pi}}\, {cgammaw}+{cbeta}\, \left({{\pi}}-{{\pi}}\, {cgammaw}\right)-{w1}\, \left({comega}\, {{u}}-100\, {epsilonw}\right)
\end{dmath}
% Equation 9
\begin{dmath}
{comega}\, {{u}}={{w}}-\left({{z}}+{epsilons}+{comega}\, {{e}}\right)
\end{dmath}
% Equation 10
\begin{dmath}
{comega}\, {{u^{n}}}=100\, {epsilonw}
\end{dmath}
% Equation 11
\begin{dmath}
{{l}}={{u}}+{{e}}
\end{dmath}
% Equation 12
\begin{dmath}
{{z}}={{z}}\, \left(1-{cv}\right)+\frac{{cv}}{1-\frac{{ch}}{{ctau}}}\, \left({{c}}-{{c}}\, \frac{{ch}}{{ctau}}\right)
\end{dmath}
% Equation 13
\begin{dmath}
{{\bar{k}}}={{\bar{k}}}\, {k1}+{{i}}\, \left(1-{k1}\right)+{epsilonq}\, {k2}
\end{dmath}
% Equation 14
\begin{dmath}
{{k}}={{v}}+{{\bar{k}}}
\end{dmath}
% Equation 15
\begin{dmath}
{{v}}={{r^{k}}}\, \frac{1-{cpsi}}{{cpsi}}
\end{dmath}
% Equation 16
\begin{dmath}
{{k}}={{n}}+{{w}}-{{r^{k}}}
\end{dmath}
% Equation 17
\begin{dmath}
{{r}}={{r}}\, {crhointr}+\left(1-{crhointr}\right)\, \left({{\pi}}\, {crpi}+{cry}\, {{y^{gap}}}\right)-{epsilonr}
\end{dmath}
% Equation 18
\begin{dmath}
0={e1}\, \left({{n}}-{{e}}\right)
\end{dmath}
% Equation 19
\begin{dmath}
{cf}={c1}\, {cf}+\left(1-{c1}\right)\, {cf}-{c2}\, \left({rf}-{epsilonb}\right)
\end{dmath}
% Equation 20
\begin{dmath}
{invf}={epsilonq}+{i1}\, {invf}+\left(1-{i1}\right)\, {invf}+{i2}\, {qf}
\end{dmath}
% Equation 21
\begin{dmath}
{qf}={q1}\, {rkf}-\left({rf}-{epsilonb}\right)+\left(1-{q1}\right)\, {qf}
\end{dmath}
% Equation 22
\begin{dmath}
{yf}={epsilong}+{ccy}\, {cf}+{ciy}\, {invf}+{cvy}\, {vf}
\end{dmath}
% Equation 23
\begin{dmath}
{yf}={cpsip}\, \left({epsilona}+{calpha}\, {kf}+\left(1-{calpha}\right)\, {nf}\right)
\end{dmath}
% Equation 24
\begin{dmath}
0=\left(1-{calpha}\right)\, {wf}+{calpha}\, {rkf}-{epsilona}
\end{dmath}
% Equation 25
\begin{dmath}
{wf}={epsilons}+{zf}+{comega}\, {nf}
\end{dmath}
% Equation 26
\begin{dmath}
{zf}=\left(1-{cv}\right)\, {zf}+\frac{{cv}}{1-\frac{{ch}}{{ctau}}}\, \left({cf}-\frac{{ch}}{{ctau}}\, {cf}\right)
\end{dmath}
% Equation 27
\begin{dmath}
{kbarf}={epsilonq}\, {k2}+{k1}\, {kbarf}+\left(1-{k1}\right)\, {invf}
\end{dmath}
% Equation 28
\begin{dmath}
{kf}={vf}+{kbarf}
\end{dmath}
% Equation 29
\begin{dmath}
{vf}=\frac{1-{cpsi}}{{cpsi}}\, {rkf}
\end{dmath}
% Equation 30
\begin{dmath}
{kf}={nf}+{wf}-{rkf}
\end{dmath}
% Equation 31
\begin{dmath}
0={e1}\, \left({nf}-{ef}\right)
\end{dmath}
% Equation 32
\begin{dmath}
{{y^{gap}}}={{y}}-{yf}
\end{dmath}
% Equation 33
\begin{dmath}
{epsilonb}={epsilonb}\, {crhob}+{etab}
\end{dmath}
% Equation 34
\begin{dmath}
{epsilonq}={epsilonq}\, {crhoq}+{etaq}
\end{dmath}
% Equation 35
\begin{dmath}
{epsilong}={epsilong}\, {crhog}+{etag}+{crhoga}\, {etaa}
\end{dmath}
% Equation 36
\begin{dmath}
{epsilona}={etaa}+{epsilona}\, {crhoa}
\end{dmath}
% Equation 37
\begin{dmath}
{epsilonp}={epsilonp}\, {crhop}+{etap}-{cmup}\, {AUX\_EXO\_LAG\_54\_0}
\end{dmath}
% Equation 38
\begin{dmath}
{epsilonr}={epsilonr}\, {crhor}+{etar}
\end{dmath}
% Equation 39
\begin{dmath}
{epsilons}={epsilons}\, {crhos}+{etas}
\end{dmath}
% Equation 40
\begin{dmath}
{epsilonw}={epsilonw}\, {crhow}+{etaw}-{cmuw}\, {AUX\_EXO\_LAG\_56\_0}
\end{dmath}
% Equation 41
\begin{dmath}
{dyobs}={ctaubar}+{cebar}
\end{dmath}
% Equation 42
\begin{dmath}
{dcobs}={ctaubar}+{cebar}
\end{dmath}
% Equation 43
\begin{dmath}
{diobs}={ctaubar}+{cebar}
\end{dmath}
% Equation 44
\begin{dmath}
{piobs}={{\pi}}+{cpibar}
\end{dmath}
% Equation 45
\begin{dmath}
{dwobs}-{piobs}={ctaubar}
\end{dmath}
% Equation 46
\begin{dmath}
{deobs}={cebar}
\end{dmath}
% Equation 47
\begin{dmath}
{uobs}={{u}}+{cubar}
\end{dmath}
% Equation 48
\begin{dmath}
{robs}=4\, {crbar}+{{r}}\, 4
\end{dmath}
% Equation 49
\begin{dmath}
{ryear}={{r}}\, 4
\end{dmath}
% Equation 50
\begin{dmath}
{piyear}={{\pi}}+{{\pi}}+{AUX\_ENDO\_LAG\_2\_1}+{AUX\_ENDO\_LAG\_2\_2}
\end{dmath}
% Equation 51
\begin{dmath}
{AUX\_ENDO\_LAG\_2\_1}={{\pi}}
\end{dmath}
% Equation 52
\begin{dmath}
{AUX\_ENDO\_LAG\_2\_2}={AUX\_ENDO\_LAG\_2\_1}
\end{dmath}
% Equation 53
\begin{dmath}
{AUX\_EXO\_LAG\_54\_0}={etap}
\end{dmath}
% Equation 54
\begin{dmath}
{AUX\_EXO\_LAG\_56\_0}={etaw}
\end{dmath}
