% Equation 1
\begin{dmath}
{{c}}_{t}={{c_1}}\, {{c}}_{t+1}+\left(1-{{c_1}}\right)\, {{c}}_{t-1}-{{c_2}}\, \left({{r}}_{t}-{{\pi}}_{t+1}-{{\varepsilon_b}}_{t}\right)
\end{dmath}
% Equation 2
\begin{dmath}
{{i}}_{t}={{i_1}}\, {{i}}_{t-1}+\left(1-{{i_1}}\right)\, {{i}}_{t+1}+{{i_2}}\, {{q}}_{t}+{{\varepsilon_q}}_{t}
\end{dmath}
% Equation 3
\begin{dmath}
{{q}}_{t}={{q_1}}\, {{r^{k}}}_{t+1}-\left({{r}}_{t}-{{\pi}}_{t+1}-{{\varepsilon_b}}_{t}\right)+\left(1-{{q_1}}\right)\, {{q}}_{t+1}
\end{dmath}
% Equation 4
\begin{dmath}
{{y}}_{t}={{c}}_{t}\, {{\frac{\bar{c}}{y}}}+{{i}}_{t}\, {{\frac{\bar{i}}{y}}}+{{\frac{\bar{v}}{y}}}\, {{v}}_{t}+{{\varepsilon_g}}_{t}
\end{dmath}
% Equation 5
\begin{dmath}
{{y}}_{t}={{\psi_p}}\, \left({{\alpha}}\, {{k}}_{t}+\left(1-{{\alpha}}\right)\, {{n}}_{t}+{{\varepsilon_a}}_{t}\right)
\end{dmath}
% Equation 6
\begin{dmath}
{{\pi}}_{t}={{w_{energy}}}\, {{\pi_energy}}_{t}+{{w_{food}}}\, {{\pi_fodd}}_{t}+\left(1-{{w_{energy}}}-{{w_{food}}}\right)\, {{\pi_core}}_{t}
\end{dmath}
% Equation 7
\begin{dmath}
{{\pi_core}}_{t}-{{\gamma_p}}\, {{\pi_core}}_{t-1}={{\pi_1}}\, \left({{\pi_core}}_{t+1}-{{\pi_core}}_{t}\, {{\gamma_p}}\right)-{{\pi_2}}\, \left(100\, {{\varepsilon_p}}_{t}-{{mc}}_{t}\right)
\end{dmath}
% Equation 8
\begin{dmath}
{{\pi_fodd}}_{t}-{{\gamma_p}}\, {{\pi_fodd}}_{t-1}={{\pi_1}}\, \left({{\pi_fodd}}_{t+1}-{{\pi_fodd}}_{t}\, {{\gamma_p}}\right)-{{\pi_2}}\, \left(100\, {{\varepsilon_p}}_{t}-{{mc}}_{t}+100\, {{\varepsilon_p^{food}}_{t}\right)
\end{dmath}
% Equation 9
\begin{dmath}
{{\pi_energy}}_{t}-{{\gamma_p}}\, {{\pi_energy}}_{t-1}={{\pi_1}}\, \left({{\pi_energy}}_{t+1}-{{\pi_energy}}_{t}\, {{\gamma_p}}\right)-{{\pi_2}}\, \left(100\, {{\varepsilon_p}}_{t}-{{mc}}_{t}+100\, {{\varepsilon_p^{energy}}}_{t}\right)
\end{dmath}
% Equation 10
\begin{dmath}
{{mc}}_{t}=\left(1-{{\alpha}}\right)\, {{w}}_{t}+{{\alpha}}\, {{r^{k}}}_{t}-{{\varepsilon_a}}_{t}
\end{dmath}
% Equation 11
\begin{dmath}
{{\pi}}_{t}+{{w}}_{t}-{{w}}_{t-1}={{\gamma_w}}\, {{\pi}}_{t-1}+{{\beta}}\, \left({{\pi}}_{t+1}+{{w}}_{t+1}-{{w}}_{t}-{{\pi}}_{t}\, {{\gamma_w}}\right)-{{w_1}}\, \left({{\omega}}\, {{u}}_{t}-100\, {{\varepsilon_w}}_{t}\right)
\end{dmath}
% Equation 12
\begin{dmath}
{{\omega}}\, {{u}}_{t}={{w}}_{t}-\left({{z}}_{t}+{{\varepsilon_s}}_{t}+{{\omega}}\, {{e}}_{t}\right)
\end{dmath}
% Equation 13
\begin{dmath}
{{\omega}}\, {{u^{n}}}_{t}=100\, {{\varepsilon_w}}_{t}
\end{dmath}
% Equation 14
\begin{dmath}
{{l}}_{t}={{u}}_{t}+{{e}}_{t}
\end{dmath}
% Equation 15
\begin{dmath}
{{z}}_{t}=\left(1-{{v}}\right)\, {{z}}_{t-1}+\frac{{{v}}}{1-\frac{{{h}}}{{{\tau}}}}\, \left({{c}}_{t}-{{c}}_{t-1}\, \frac{{{h}}}{{{\tau}}}\right)
\end{dmath}
% Equation 16
\begin{dmath}
{{\bar{k}}}_{t}={{k_1}}\, {{\bar{k}}}_{t-1}+{{i}}_{t}\, \left(1-{{k_1}}\right)+{{\varepsilon_q}}_{t}\, {{k_2}}
\end{dmath}
% Equation 17
\begin{dmath}
{{k}}_{t}={{v}}_{t}+{{\bar{k}}}_{t-1}
\end{dmath}
% Equation 18
\begin{dmath}
{{v}}_{t}={{r^{k}}}_{t}\, \frac{1-{{\psi}}}{{{\psi}}}
\end{dmath}
% Equation 19
\begin{dmath}
{{k}}_{t}={{n}}_{t}+{{w}}_{t}-{{r^{k}}}_{t}
\end{dmath}
% Equation 20
\begin{dmath}
{{r}}_{t}={{\rho_{i}}}\, {{r}}_{t-1}+\left(1-{{\rho_{i}}}\right)\, \left({{\pi}}_{t}\, {{r_{\pi}}}+{{r_{y}}}\, {{y^{gap}}}_{t}+{{r_{\Delta y}}}\, \left({{y^{gap}}}_{t}-{{y^{gap}}}_{t-1}\right)\right)-{{\varepsilon_r}}_{t}
\end{dmath}
% Equation 21
\begin{dmath}
{{e}}_{t}-{{e}}_{t-1}={{\beta}}\, \left({{e}}_{t+1}-{{e}}_{t}\right)+{{e_1}}\, \left({{n}}_{t}-{{e}}_{t}\right)
\end{dmath}
% Equation 22
\begin{dmath}
{{c^{f}}}_{t}={{c_1}}\, {{c^{f}}}_{t+1}+\left(1-{{c_1}}\right)\, {{c^{f}}}_{t-1}-{{c_2}}\, \left({{r^{f}}}_{t}-{{\varepsilon_b}}_{t}\right)
\end{dmath}
% Equation 23
\begin{dmath}
{{i^{f}}}_{t}={{\varepsilon_q}}_{t}+{{i_1}}\, {{i^{f}}}_{t-1}+\left(1-{{i_1}}\right)\, {{i^{f}}}_{t+1}+{{i_2}}\, {{q^{f}}}_{t}
\end{dmath}
% Equation 24
\begin{dmath}
{{q^{f}}}_{t}={{q_1}}\, {{r^{k,f}}}_{t+1}-\left({{r^{f}}}_{t}-{{\varepsilon_b}}_{t}\right)+\left(1-{{q_1}}\right)\, {{q^{f}}}_{t+1}
\end{dmath}
% Equation 25
\begin{dmath}
{{y^{f}}}_{t}={{\varepsilon_g}}_{t}+{{\frac{\bar{c}}{y}}}\, {{c^{f}}}_{t}+{{\frac{\bar{i}}{y}}}\, {{i^{f}}}_{t}+{{\frac{\bar{v}}{y}}}\, {{v^{f}}}_{t}
\end{dmath}
% Equation 26
\begin{dmath}
{{y^{f}}}_{t}={{\psi_p}}\, \left({{\varepsilon_a}}_{t}+{{\alpha}}\, {{k^{f}}}_{t}+\left(1-{{\alpha}}\right)\, {{n^{f}}}_{t}\right)
\end{dmath}
% Equation 27
\begin{dmath}
0=\left(1-{{\alpha}}\right)\, {{w^{f}}}_{t}+{{\alpha}}\, {{r^{k,f}}}_{t}-{{\varepsilon_a}}_{t}
\end{dmath}
% Equation 28
\begin{dmath}
{{w^{f}}}_{t}={{\varepsilon_s}}_{t}+{{z^{f}}}_{t}+{{\omega}}\, {{n^{f}}}_{t}
\end{dmath}
% Equation 29
\begin{dmath}
{{z^{f}}}_{t}=\left(1-{{v}}\right)\, {{z^{f}}}_{t-1}+\frac{{{v}}}{1-\frac{{{h}}}{{{\tau}}}}\, \left({{c^{f}}}_{t}-\frac{{{h}}}{{{\tau}}}\, {{c^{f}}}_{t-1}\right)
\end{dmath}
% Equation 30
\begin{dmath}
{{\bar{k}^{f}}}_{t}={{\varepsilon_q}}_{t}\, {{k_2}}+{{k_1}}\, {{\bar{k}^{f}}}_{t-1}+\left(1-{{k_1}}\right)\, {{i^{f}}}_{t}
\end{dmath}
% Equation 31
\begin{dmath}
{{k^{f}}}_{t}={{v^{f}}}_{t}+{{\bar{k}^{f}}}_{t-1}
\end{dmath}
% Equation 32
\begin{dmath}
{{v^{f}}}_{t}=\frac{1-{{\psi}}}{{{\psi}}}\, {{r^{k,f}}}_{t}
\end{dmath}
% Equation 33
\begin{dmath}
{{k^{f}}}_{t}={{n^{f}}}_{t}+{{w^{f}}}_{t}-{{r^{k,f}}}_{t}
\end{dmath}
% Equation 34
\begin{dmath}
{{e^{f}}}_{t}-{{e^{f}}}_{t-1}={{\beta}}\, \left({{e^{f}}}_{t+1}-{{e^{f}}}_{t}\right)+{{e_1}}\, \left({{n^{f}}}_{t}-{{e^{f}}}_{t}\right)
\end{dmath}
% Equation 35
\begin{dmath}
{{y^{gap}}}_{t}={{y}}_{t}-{{y^{f}}}_{t}
\end{dmath}
% Equation 36
\begin{dmath}
{{\varepsilon_a}}_{t}={{\rho_a}}\, {{\varepsilon_a}}_{t-1}+{{\eta_a}}_{t}
\end{dmath}
% Equation 37
\begin{dmath}
{{\varepsilon_b}}_{t}={{\rho_b}}\, {{\varepsilon_b}}_{t-1}+{{\eta_b}}_{t}
\end{dmath}
% Equation 38
\begin{dmath}
{{\varepsilon_g}}_{t}={{\rho_g}}\, {{\varepsilon_g}}_{t-1}+{{\eta_g}}_{t}+{{\eta_a}}_{t}\, {{\rho_{ga}}}
\end{dmath}
% Equation 39
\begin{dmath}
{{\varepsilon_p}}_{t}={{\rho_p}}\, {{\varepsilon_p}}_{t-1}+{{\eta_p}}_{t}-{{\mu_p}}\, {AUX\_EXO\_LAG\_62\_0}_{t-1}
\end{dmath}
% Equation 40
\begin{dmath}
{{\varepsilon_q}}_{t}={{\rho_q}}\, {{\varepsilon_q}}_{t-1}+{{\eta_q}}_{t}
\end{dmath}
% Equation 41
\begin{dmath}
{{\varepsilon_r}}_{t}={{\rho_r}}\, {{\varepsilon_r}}_{t-1}+{{\eta_r}}_{t}
\end{dmath}
% Equation 42
\begin{dmath}
{{\varepsilon_s}}_{t}={{\rho_s}}\, {{\varepsilon_s}}_{t-1}+{{\eta_s}}_{t}
\end{dmath}
% Equation 43
\begin{dmath}
{{\varepsilon_w}}_{t}={{\rho_w}}\, {{\varepsilon_w}}_{t-1}+{{\eta_w}}_{t}-{{\mu_w}}\, {AUX\_EXO\_LAG\_64\_0}_{t-1}
\end{dmath}
% Equation 44
\begin{dmath}
{{\varepsilon_p^{energy}}}_{t}={{\eta_p^{energy}}}_{t}+{{\eta_p}}_{t}+{{\rho_p^{energy}}}\, {{\varepsilon_p^{energy}}}_{t-1}-{{\mu_p}}\, {AUX\_EXO\_LAG\_62\_0}_{t-1}
\end{dmath}
% Equation 45
\begin{dmath}
{{\varepsilon_p^{food}}_{t}={{\eta_p^{food}}}_{t}+{{\eta_p}}_{t}+{{\rho_p^{food}}}\, {{\varepsilon_p^{food}}_{t-1}-{{\mu_p}}\, {AUX\_EXO\_LAG\_62\_0}_{t-1}
\end{dmath}
% Equation 46
\begin{dmath}
{{\Delta y^{obs}}}_{t}={{y}}_{t}+{{\bar{\tau}}}+{{\bar{e}}}-{{y}}_{t-1}
\end{dmath}
% Equation 47
\begin{dmath}
{{\Delta c^{obs}}}_{t}={{c}}_{t}+{{\bar{\tau}}}+{{\bar{e}}}-{{c}}_{t-1}
\end{dmath}
% Equation 48
\begin{dmath}
{{\Delta i^{obs}}}_{t}={{i}}_{t}+{{\bar{\tau}}}+{{\bar{e}}}-{{i}}_{t-1}
\end{dmath}
% Equation 49
\begin{dmath}
{{\pi^{obs}_core}}_{t}={{\pi_core}}_{t}+{{\bar{\pi}}}
\end{dmath}
% Equation 50
\begin{dmath}
{{\pi^{obs}_energy}}_{t}={{\pi_energy}}_{t}+{{\bar{\pi}}}
\end{dmath}
% Equation 51
\begin{dmath}
{{\pi^{obs}_food}}_{t}={{\pi_fodd}}_{t}+{{\bar{\pi}}}
\end{dmath}
% Equation 52
\begin{dmath}
{{\pi^{obs}}}_{t}={{w_{energy}}}\, {{\pi^{obs}_energy}}_{t}+{{w_{food}}}\, {{\pi^{obs}_food}}_{t}+\left(1-{{w_{energy}}}-{{w_{food}}}\right)\, {{\pi^{obs}_core}}_{t}
\end{dmath}
% Equation 53
\begin{dmath}
{{\Delta w^{obs}}}_{t}-{{\pi^{obs}}}_{t}={{w}}_{t}+{{\bar{\tau}}}-{{w}}_{t-1}-\left({{\pi}}_{t}-{{\pi}}_{t-1}\right)
\end{dmath}
% Equation 54
\begin{dmath}
{{\Delta e^{obs}}}_{t}={{e}}_{t}+{{\bar{e}}}-{{e}}_{t-1}
\end{dmath}
% Equation 55
\begin{dmath}
{{u^{obs}}}_{t}={{u}}_{t}+{{\bar{u}}}
\end{dmath}
% Equation 56
\begin{dmath}
{{r^{obs}}}_{t}=4\, {{\bar{r}}}+{{r}}_{t}\, 4
\end{dmath}
% Equation 57
\begin{dmath}
{{r^{ann}}}_{t}={{r}}_{t}\, 4
\end{dmath}
% Equation 58
\begin{dmath}
{{\pi^{ann}}}_{t}={{\pi}}_{t}+{{\pi}}_{t-1}+{AUX\_ENDO\_LAG\_2\_1}_{t-1}+{AUX\_ENDO\_LAG\_2\_2}_{t-1}
\end{dmath}
% Equation 59
\begin{dmath}
{AUX\_ENDO\_LAG\_2\_1}_{t}={{\pi}}_{t-1}
\end{dmath}
% Equation 60
\begin{dmath}
{AUX\_ENDO\_LAG\_2\_2}_{t}={AUX\_ENDO\_LAG\_2\_1}_{t-1}
\end{dmath}
% Equation 61
\begin{dmath}
{AUX\_EXO\_LAG\_62\_0}_{t}={{\eta_p}}_{t}
\end{dmath}
% Equation 62
\begin{dmath}
{AUX\_EXO\_LAG\_64\_0}_{t}={{\eta_w}}_{t}
\end{dmath}
